new labels and theories

theories/prob_eff_lang/probblaze/examples/DH_KE/equiv_schannel.v
@@ -21,7 +21,7 @@ Import valgroup_tactics.
 
 Section s_channel_verification.
   Context `{probblazeRGS Σ}.
-  Context (channel1 channel2 getKey1 getKey2 leak1 leak2 : label).
+  Context (channel1 channel2 getKey1 getKey2 leak1 leak2 leak'1 leak'2 schannel1 schannel2: label).
   Context {vg: val_group}.
   Context {cg: clutch_group_struct}.
   Context {G : clutch_group (vg:=vg) (cg:=cg)}.
@@ -29,36 +29,39 @@ Section s_channel_verification.
   Context `{!inG Σ (exclR unitO), !inG Σ dfracO, !inG Σ (dfrac_agreeR valO)}.
 
 
+  Definition atokN' : namespace := nroot .@ "atokN1".
+  Definition btokN' : namespace := nroot .@ "btokN1".
+
   (*Theories for the interaction of the secure channel with the environment*)
   (*-------------------------------------------------------------*)
    Program Definition SendSecBob : iThy Σ :=
   λ e1 e2, (λne Q,
-              ∀ m1 m2 : val,
-                ⌜e1 = (do: channel1 (SendV (m1, bob)))⌝%E ∗ 
-                           ⌜ e2 = do: channel2 (SendV (m2, bob)) ⌝%E ∗
+              ∃ m1 m2 : val,
+                ⌜e1 = (do: leak'1 (SendV (m1, bob)))⌝%E ∗ 
+                           ⌜ e2 = do: leak'2 (SendV (m2, bob)) ⌝%E ∗
                                       □ Q (Val #()%V) (Val #()%V))%I.
   Next Obligation. solve_proper. Qed.
 
   Program Definition SendSecAlice : iThy Σ :=
   λ e1 e2, (λne Q,
-              ∀ m1 m2 : val,
-                ⌜e1 = (do: channel1 (SendV (m1, alice)))⌝%E ∗ 
-                           ⌜ e2 = do: channel2 (SendV (m2, alice)) ⌝%E ∗
+              ∃ m1 m2 : val,
+                ⌜e1 = (do: leak'1 (SendV (m1, alice)))⌝%E ∗ 
+                           ⌜ e2 = do: leak'2 (SendV (m2, alice)) ⌝%E ∗
                                       □ Q (Val #()%V) (Val #()%V))%I.
   Next Obligation. solve_proper. Qed.
 
   Program Definition RecvSecBob : iThy Σ :=
    λ e1 e2, (λne Q,
-                ⌜ e1 = do: channel1 (RecvV bob) ⌝%E ∗
-                ⌜ e2 = do: channel2 (RecvV bob) ⌝%E ∗
+                ⌜ e1 = do: leak'1 (RecvV bob) ⌝%E ∗
+                ⌜ e2 = do: leak'2 (RecvV bob) ⌝%E ∗
                 □ ((∀ b1 b2 : nat, Q (SOMEV #b1) (SOMEV #b2)) ∧ Q NONEV NONEV)
              )%I.
   Next Obligation. solve_proper. Qed.
 
   Program Definition RecvSecAlice : iThy Σ :=
      λ e1 e2, (λne Q,
-                ⌜ e1 = do: channel1 (RecvV alice) ⌝%E ∗
-                ⌜ e2 = do: channel2 (RecvV alice) ⌝%E ∗
+                ⌜ e1 = do: leak'1 (RecvV alice) ⌝%E ∗
+                ⌜ e2 = do: leak'2 (RecvV alice) ⌝%E ∗
                 □ ((∀ b1 b2 : nat, Q (SOMEV #b1) (SOMEV #b2)) ∧ Q NONEV NONEV)
              )%I.
   Next Obligation. solve_proper. Qed.
@@ -77,17 +80,16 @@ Section s_channel_verification.
                                       □ Q (Val #()%V) (Val #()%V))%I.
   Next Obligation. solve_proper. Qed.
 
-  
 
-  Definition LblEnvSec := [([channel1], [channel2],iThySum (iThySum SendSecBob RecvSecAlice) (iThySum RecvSecBob RecvSecAlice)); ([leak1], [leak2], iThySum LeakAlice LeakBob)].
+  Definition LblEnvSec := [ ([channel1; getKey1; schannel1], [channel2; schannel2], iThyBot)    ; ([leak'1], [leak'2],iThySum (iThySum SendSecBob RecvSecAlice) (iThySum RecvSecBob RecvSecAlice)); ([leak1], [leak2], iThySum LeakAlice LeakBob)].
 
   (*Theories for the implementation of the secure channel*)
   (*---------------------------------------------------------*)
    Program Definition SendSecBobImpl γtok γfrac γsec ℓ : iThy Σ :=
      λ e1 e2, (λne Q,
                 ∃ m m': val, ((|={⊤, ⊤ ∖ ↑ℓ }=> ((own γfrac DfracDiscarded -∗ (|={⊤ ∖ ↑ℓ, ⊤}=> token γtok ∗ own γsec (to_dfrac_agree DfracDiscarded m) ∗ ⌜m = m'⌝)) ∨ |={⊤ ∖ ↑ℓ , ⊤}=> own γfrac DfracDiscarded)) ∗  
-                            (⌜ e1 = do: channel1 (SendV (m, alice)) ⌝%E ∗
-                             ⌜ e2 = do: channel2 (SendV (m', alice)) ⌝%E)  ∗ 
+                            (⌜ e1 = do: schannel1 (SendV (m, alice)) ⌝%E ∗
+                             ⌜ e2 = do: schannel2 (SendV (m', alice)) ⌝%E)  ∗ 
                             □ (Q (Val #()%V) (Val #()%V)))
              )%I.
   Next Obligation. solve_proper. Qed.
@@ -95,67 +97,285 @@ Section s_channel_verification.
   Program Definition SendSecAliceImpl γtok γfrac γsec ℓ : iThy Σ :=
      λ e1 e2, (λne Q,
                 ∃ m m' : val, ((|={⊤, ⊤ ∖ ↑ℓ }=> ((own γfrac DfracDiscarded -∗ (|={⊤ ∖ ↑ℓ, ⊤}=> token γtok ∗ own γsec (to_dfrac_agree DfracDiscarded m) ∗ ⌜m = m'⌝)) ∨ |={⊤ ∖ ↑ℓ , ⊤}=> own γfrac DfracDiscarded)) ∗  
-                             (⌜ e1 = do: channel1 (SendV (m, bob)) ⌝%E ∗
-                              ⌜ e2 = do: channel2 (SendV (m', bob)) ⌝%E)  ∗ 
+                             (⌜ e1 = do: schannel1 (SendV (m, bob)) ⌝%E ∗
+                              ⌜ e2 = do: schannel2 (SendV (m', bob)) ⌝%E)  ∗ 
                              □ (Q (Val #()%V) (Val #()%V)))
              )%I.
   Next Obligation. solve_proper. Qed.
   
   Program Definition RecvSecBobImpl γsec : iThy Σ :=
      λ e1 e2, (λne Q,
-                ⌜ e1 = do: channel1 (RecvV bob) ⌝%E ∗
-                ⌜ e2 = do: channel2 (RecvV bob) ⌝%E ∗
+                ⌜ e1 = do: schannel1 (RecvV bob) ⌝%E ∗
+                ⌜ e2 = do: schannel2 (RecvV bob) ⌝%E ∗
                 □ (Q NONEV NONEV ∗ (∀ m, own γsec (to_dfrac_agree DfracDiscarded m) -∗ Q (SOMEV m) (SOMEV m)))
              )%I.
   Next Obligation. solve_proper. Qed. 
     
   Program Definition RecvSecAliceImpl γsec : iThy Σ :=
      λ e1 e2, (λne Q,
-                 ⌜ e1 = do: channel1 (RecvV alice) ⌝%E ∗
-                 ⌜ e2 = do: channel2 (RecvV alice) ⌝%E ∗
+                 ⌜ e1 = do: schannel1 (RecvV alice) ⌝%E ∗
+                 ⌜ e2 = do: schannel2 (RecvV alice) ⌝%E ∗
                  □ (Q NONEV NONEV ∗ (∀ m, own γsec (to_dfrac_agree DfracDiscarded m) -∗ Q (SOMEV m) (SOMEV m)))
              )%I.
   Next Obligation. solve_proper. Qed.
 
 
 
-  Definition LblSecChannel γtoka atokN γfraca γseca γsecb : iLblThy Σ :=
-    [([channel1],[channel2], (iThySum (SendSecAliceImpl γtoka γfraca γseca atokN) (RecvSecBobImpl γsecb)))].
+  (*Definition LblSecChannel γtoka atokN γfraca γseca γsecb : iLblThy Σ :=
+    [([channel1; getKey1],[channel2], (iThySum (SendSecAliceImpl γtoka γfraca γseca atokN) (RecvSecBobImpl γsecb)))].*)
   (*    (iThySum (SendSecBobImpl γtokb γfracb γsecb btokN) (RecvSecAliceImpl γseca))))].*)
+  Definition SecChannelThy  γtoka atokN' γfraca γseca γsecb : iThy Σ :=
+    (iThySum (SendSecAliceImpl γtoka γfraca γseca atokN') (RecvSecBobImpl γsecb)).
 
 
+  Program Definition SendAuthBobImpl γtok γfrac γauth ι : iThy Σ :=
+    λ e1 e2, (λne Q,
+                ∃ m m': val, ((|={⊤, ⊤ ∖ ↑ι }=> ((own γfrac DfracDiscarded -∗ (|={⊤ ∖ ↑ι, ⊤}=> token γtok ∗ own γauth (to_dfrac_agree DfracDiscarded m) ∗ ⌜m = m'⌝)) ∨ |={⊤ ∖ ↑ι , ⊤}=> own γfrac DfracDiscarded)) ∗  
+                            (⌜ e1 = do: channel1 (SendV (m, alice)) ⌝%E ∗
+                             ⌜ e2 = do: channel2 (SendV (m', alice)) ⌝%E)  ∗ 
+                            □ (Q (Val #()%V) (Val #()%V)))
+             )%I.
+  Next Obligation. solve_proper. Qed.
+
+  Program Definition RecvAuthAliceImpl γauth : iThy Σ :=
+    λ e1 e2, (λne Q,
+                 ⌜ e1 = do: channel1 (RecvV alice) ⌝%E ∗
+                 ⌜ e2 = do: channel2 (RecvV alice) ⌝%E ∗
+                 □ (Q NONEV NONEV ∗ (∀ m, own γauth (to_dfrac_agree DfracDiscarded m) -∗ Q (SOMEV m) (SOMEV m)))
+             )%I.
+  Next Obligation. solve_proper. Qed.
+
+   Program Definition SendAuthAliceImpl γtok γfrac γauth ι : iThy Σ :=
+    λ e1 e2, (λne Q,
+                ∃ m m' : val, ((|={⊤, ⊤ ∖ ↑ι }=> ((own γfrac DfracDiscarded -∗ (|={⊤ ∖ ↑ι, ⊤}=> token γtok ∗ own γauth (to_dfrac_agree DfracDiscarded m) ∗ ⌜m = m'⌝)) ∨ |={⊤ ∖ ↑ι , ⊤}=> own γfrac DfracDiscarded)) ∗  
+                             (⌜ e1 = do: channel1 (SendV (m, bob)) ⌝%E ∗
+                              ⌜ e2 = do: channel2 (SendV (m', bob)) ⌝%E)  ∗ 
+                             □ (Q (Val #()%V) (Val #()%V)))
+             )%I.
+   Next Obligation. solve_proper. Qed.
+
+
+   Program Definition RecvAuthBobImpl γauth : iThy Σ :=
+    λ e1 e2, (λne Q,
+                ⌜ e1 = do: channel1 (RecvV bob) ⌝%E ∗
+                ⌜ e2 = do: channel2 (RecvV bob) ⌝%E ∗
+                □ (Q NONEV NONEV ∗ (∀ m, own γauth (to_dfrac_agree DfracDiscarded m) -∗ Q (SOMEV m) (SOMEV m)))
+             )%I.
+  Next Obligation. solve_proper. Qed. 
+
+   
+  Definition AuthChannelThy γtoka atokN γtokb btokN γfraca γfracb γautha γauthb : iThy Σ :=
+    (iThySum (iThySum (SendAuthAliceImpl γtoka γfraca γautha atokN) (RecvAuthBobImpl γauthb))
+                                (iThySum (SendAuthBobImpl γtokb γfracb γauthb btokN) (RecvAuthAliceImpl γautha))).
+  Definition ClientThy γtoka atokN γfraca γseca γsecb γtoka1 γtokb1 γfraca1 γfracb1 γautha γauthb atokN1 btokN1  : iThy Σ :=
+    (iThySum (SecChannelThy γtoka atokN γfraca γseca γsecb) (AuthChannelThy γtoka1 atokN1 γtokb1 btokN1 γfraca1 γfracb1 γautha
+    γauthb)).
+  Definition LblClients γtoka atokN γfraca γseca γsecb γtoka1 γtokb1 γfraca1 γfracb1 γautha γauthb atokN1 btokN1 : iLblThy Σ :=
+    [([schannel1; getKey1; channel1],[schannel2; channel2], ClientThy γtoka atokN γfraca γseca γsecb γtoka1 γtokb1 γfraca1 γfracb1 γautha γauthb atokN1 btokN1)].
+  
 (*Verification of F_OAUTH[F_KE_L[CHAN[]]] ≤ CHAN_SIM[F_CHAN[]]*)
 (*----------------------------------------------------------*)
-Lemma F_KE_CHAN_SIM f1 f2 γtoka γfraca γseca γsecb L :
-    let LblThy := LblSecChannel γtoka atokN γfraca γseca γsecb in
+Lemma F_KE_CHAN_SIM f1 f2 γtoka atokN γfraca γseca γsecb γtoka1 γtokb1 γfraca1 γfracb1 γautha γauthb atokN1 btokN1 L :
+  let LblThy := LblClients γtoka atokN γfraca γseca γsecb γtoka1 γtokb1 γfraca1 γfracb1 γautha γauthb atokN1 btokN1 in
+  let Xthy := iThySum (iThySum SendSecBob RecvSecAlice)
+        (iThySum RecvSecBob RecvSecAlice) in 
     is_closed_expr ∅ f1 ->
     is_closed_expr ∅ f2 ->
     token γtoka -∗ 
-    (*token γtokb -**)
+    token γtoka1 -∗
+    token γtokb1 -∗
     own γseca (to_dfrac_agree (DfracOwn 1) #()%V) -∗ 
-    own γsecb (to_dfrac_agree (DfracOwn 1) #()%V) -∗ 
+    own γsecb (to_dfrac_agree (DfracOwn 1) #()%V) -∗
+    own γautha (to_dfrac_agree (DfracOwn 1) #()%V) -∗ 
+    own γauthb (to_dfrac_agree (DfracOwn 1) #()%V) -∗ 
     BREL f1 ≤ f2 <| LblThy ++ L |> {{ (λ v1 v2, ⌜ v1 = v2 ⌝)  }} -∗ 
-    BREL (F_OAUTH channel1 (F_KE_L getKey1 channel1 leak1 (CHAN getKey1 channel1 f1)))
-    ≤ CHAN_SIM channel2 leak2 (F_CHAN channel2 f2)<| LblEnvSec ++ L |> {{ (λ v1 v2, ⌜ v1 = v2 ⌝) }}.
+    BREL (F_OAUTH leak'1 channel1 (F_KE_L getKey1 channel1 leak1 (CHAN getKey1 schannel1 channel1 f1)))
+    ≤ CHAN_SIM leak'2 leak2 channel2 (F_CHAN schannel2 channel2 f2)<| LblEnvSec ++ L |> {{ (λ v1 v2, ⌜ v1 = v2 ⌝) }}.
 Proof with (repeat foldkont) using G.
-  iIntros (LblThy Hf1 Hf2) "Htoka Howna Hownb Hf1f2".
-  iApply brel_alloctape_r. iIntros (α) "Hα". brel_pures_r.
+  iIntros (LblThy Xthy Hf1 Hf2) "Htoka Htoka1 Htokb1 Hsecowna Hsecownb Hauthowna Hauthownb Hf1f2". repeat simpl. 
+  iApply brel_alloctape_r. iIntros (β) "Hβ". brel_pures_r. 
   iApply brel_alloc_r. iIntros (l2) "Hl2". brel_pures_r.
   iApply brel_alloc_l. iIntros (l1) "!>Hl1". brel_pures_l.
   rewrite subst_is_closed_empty; try done.
-  iApply brel_alloc_r. iIntros (l0) "Hl0".
-  Search "couple" "brel".
-  iApply brel_couple_UT; try done.
-  iFrame. iSplit; first done. iIntros (n) "!>Hn Hα".
-  brel_pures_l. brel_exp_l. brel_pures_l. iApply brel_alloc_l.
-  iIntros (l3) "!>Hl3". brel_pures_l. repeat (rewrite subst_is_closed_empty; try done). brel_pures_r. rewrite subst_is_closed_empty; try done.
-  iApply brel_exhaustion.
-  Search "handle".
+  iApply brel_couple_UT. 1: auto.
+  simpl. iFrame "Hβ". iSplit => //.
+  iIntros (n ?) "!> Hβ". brel_pures.
+  rewrite subst_is_closed_empty; try done.
+  brel_exp_l. brel_pures.
+  iApply brel_alloc_l. iIntros (l3) "!>Hl3". brel_pures_l.
+  simpl. do 2 rewrite subst_is_closed_empty; try done.
+  iApply brel_alloc_r. iIntros (l0) "Hl0". brel_pures_r.
+  rewrite subst_is_closed_empty; try done.
+  iApply (brel_exhaustion f1 f2); try simpl. 
+  (* use update modality to change the value associated
+to the token Alic owns to the message to be sent*)
+  iApply fupd_brel.
+  set (gn := (g^+ n)%g).
+  iMod (auth_upd (vgval (g ^+n)%g) with "Howna") as "Howna".
+  iMod (auth_persist with "Howna") as "#Howna".
+  iMod (auth_persist with "Hownb") as "#Hownb".
+  iModIntro.
+
+  (*use update modality, add the token atokN to the namespace of open invariants, and then allocate an invariant corresponding to either a sample is drawn from the tape or not*)
+  (*iApply fupd_brel.
+  iMod (inv_alloc atokN _ (token γtoka ∨ own γfraca DfracDiscarded)%I with "[Htoka]") as "#Hinvta".
+  { iNext; iFrame. }
+  iModIntro.
+  iApply (brel_na_alloc
+              ((β ↪ₛN (S n''; [n]) ∗ l2 ↦ₛ NONEV)
+               ∨ (β ↪ₛ□ (S n''; [])
+                  ∗ l2 ↦ₛ□ SOMEV #n)
+              )%I
+              betaN).
+   iSplitL "Hβ Hl2"; [iNext; iFrame; iLeft; iFrame|].
+   iIntros "#Hinvn".
+   set (kl1 := (match: "payload" with
+         InjL "payload" =>
+           let: "dst" := "payload" in
+           let: "m" := Fst "dst" in
+           let: "dst" := Snd "dst" in
+           match: ! #l3 with
+             InjL <> =>
+               #l3 <- InjR "m";; 
+               let: "key" := do: getKey1 "dst" in
+               match: "key" with
+                 InjL <> => "k" (InjLV #()%V)
+               | InjR "x" => let: "enc_m" := #()%V in (do: channel1 InjL ("enc_m", bob));; "k" #()%V
+               end
+           | InjR "message" => "k" (InjLV #()%V)
+           end
+       | InjR "from" =>
+         let: "key" := do: getKey1 "from" in
+         match: "key" with
+           InjL <> => "k" (InjLV #()%V)
+         | InjR "key" =>
+           let: "r" := do: channel1 InjR "from" in
+           match: "r" with InjL <> => "k" (InjLV #()%V) | InjR "x" => let: "enc_m" := #()%V in "k" (InjR "enc_m") end
+         end
+                         end)%E).
+  set (kl2 :=  (match: "p" with
+         InjL <> =>
+           (do: leak1 bob);; 
+           let: "r" := do: channel1 InjR bob in match: "r" with InjL <> => "k" (InjLV #()%V) | InjR "w" => "k" (InjR (vgval (g ^+ n))) end
+       | InjR <> =>
+         let: "r" := do: channel1 InjR alice in
+         match: "r" with InjL <> => "k" (InjLV #()%V) | InjR "w" => (do: leak1 alice);; "k" (InjR (vgval (g ^+ n))) end
+                       end)%E).
+  set (kl3 := ( match: "payload" with
+         InjL "payload" =>
+           let: "dst" := "payload" in
+           let: "m" := Fst "dst" in
+           let: "dst" := Snd "dst" in
+           match: ! #l1 with InjL <> => #l1 <- InjR "m";; (do: channel1 InjL ("m", "dst"));; "k" #()%V | InjR "message" => "k" #()%V end
+       | InjR "from" => let: "r" := do: channel1 InjR "from" in match: "r" with InjL <> => "k" (InjLV #()%V) | InjR "x" => "k" ! #l1 end
+                                     end)%E).
+  set (kr1 :=  (match: "payload" with
+         InjL "payload" =>
+           let: "dst" := "payload" in
+           let: "m" := Fst "dst" in
+           let: "dst" := Snd "dst" in
+           match: ! #l0 with InjL <> => #l0 <- InjR "m";; (do: channel2 InjL (#0, "dst"));; "k" #()%V | InjR "x" => "k" #()%V end
+       | InjR "from" => let: "r" := do: channel2 InjR "from" in match: "r" with InjL <> => "k" (InjLV #()%V) | InjR "x" => "k" ! #l0 end
+                                     end)%E).
+  set (kr2 :=  (match: "payload" with
+         InjL "payload" =>
+           let: "dst" := "payload" in
+           let: "m" := Fst "dst" in
+           let: "dst" := Snd "dst" in
+           (do: leak2 "dst");; 
+           let: "r" := do: channel2 InjR bob in
+           match: "r" with
+             InjL <> => "k" (InjL #()%V)
+           | InjR "x" =>
+             let: "m" := match: ! #l2 with
+                           InjL <> => let: "m" := #()%V;; rand(#lbl:β) #(S n'') in #l2 <- InjR "m";; "m"
+                         | InjR "m" => "m"
+                         end in
+             let: "mA" := g ^ "m" in (do: channel2 InjL ("mA", alice));; "k" #()%V
+           end
+       | InjR "from " =>
+         let: "r" := do: channel2 InjR "from" in
+         match: "r" with InjL <> => "k" (InjL #()%V) | InjR "x" => (do: leak2 "from");; "k" (InjR #0) end
+                       end)%E).
   About brel_exhaustion.
+  Search HandleCtx.
+  Print brel_exhaustion.
+  About brel_introduction_mono.
+  Print to_iThy_le.
+  iApply (brel_exhaustion f1 f2); try simpl. 
+  About ectx_labels.
+  Print HandleCtx.
+   iApply brel_exhaustion; try set_solver...
+  1: {
+  try done.
+  iFrame "Hβ". simpl.
+  iIntros (b) "Hβ".
+  Print brel_couple_UT.
+  iIntros (n ?) "!> Hn".
+*)
+
+
+
+
+
+(*  (*-------------------------------------------------*)
+  iApply brel_alloc_r. iIntros (l0) "Hl0".
+  iApply brel_couple_UT; try done.
+  iFrame "Hα". simpl. iSplit => //. iIntros (n ?) "!> Hα".
+  (*iFrame. iSplit; first done. iIntros (n) "!>Hn Hα".*)
+  brel_pures_l. brel_exp_l. brel_pures_l. iApply brel_alloc_l.
+  iIntros (l3) "!>Hl3". brel_pures_l. repeat (rewrite subst_is_closed_empty; try done). brel_pures_r.
+  rewrite subst_is_closed_empty; try done...
+  (*Search "brel_exhaustion".
+  Search "HandleCtx".
+  About ectx.*)
+ 
+  (*iApply fupd_brel.
+   iMod (inv_alloc atokN _ (token γtoka ∨ own γfraca DfracDiscarded)%I with "[Htoka]") as "#Hinvta".
+   { iNext; iLeft;iFrame. }
+   iModIntro.
+
+    iApply (brel_na_alloc
+              ((α ↪ₛN (S n''; [n]) ∗ l2 ↦ₛ NONEV)
+               ∨ (α ↪ₛ□ (S n''; [])
+                  ∗ l2 ↦ₛ□ SOMEV #n)
+              )%I
+              alphaN).
+   iSplitL "Hα Hl2"; [iNext; iFrame; iLeft; iFrame|].
+   iIntros "#Hinvn".*)
+  iApply (brel_exhaustion _ _ [HandleCtx _ _ _ _ _] [HandleCtx _ _ _ _ _] Xthy _ _ (λ v1 v2, ⌜v1=v2⌝)%I); try done.
+  {  admit.}
+  iLöb as "IH". simpl.
+
+  iSplit; [iIntros (v1 v2) "!#Hv1v2"; brel_pures; iModIntro; done|].
+  iIntros (?????) "!# %Hk1 %Hk2 [[H1 | H1'] | [H2 | H3]] #Hrel".
+  1 : { iDestruct "H1" as (m1 m2) "[%He1 [%He2 Hqv]]".
+        rewrite He1.
+        rewrite He2. 
+        brel_pures; [apply Hk1; set_solver|apply Hk2; set_solver|]...
+        
+     iApply (brel_na_inv _ _ alphaN); first set_solver.   
+     iFrame "Hinvn".
+     iIntros "([(Hα & Hla) | (#Hα & #Hla)] & Hclose)".
+        - Print brel_load_l.
+          iApply brel_load_l.
+  iDestruct "HXQ" as " "
+  
+   (* will need induction, since send and receive can be called more than once*)
+  { iSplit.
+    + iModIntro. iIntros (v1 v2) "%Hv1v2".
+      simpl.
+      destruct v1; try (destruct v2); try (inversion Hv1v2);
+      try (brel_pures); try (iModIntro);
+        try (iPureIntro); try auto.
+    + iModIntro. iIntros (k1' k2' e1' e2' Q) "Hk1' Hk2 HXQ Hrel".
+      simpl.
+     
+  iApply (brel_exhaustion _ _ [_] [_] with "[$]").
+  iApply (brel_exhaustion _ _ [(HandleCtx Deep MS channel1 kl3 #()%V)]
+            [(HandleCtx Deep MS channel2 kr2 _)] _ _ _ _ _ _ _).
   About PureExec.
-  About unshot.
-  Search unshot.
-  About ContV.
+  About unshot.*)
 Admitted.
 
 
@@ -163,7 +383,7 @@ Admitted.
 
 (*Verification of CHAN_SIM[F_CHAN[]] ≤ F_OAUTH[F_KE_L[CHAN[]]]*)
 (*---------------------------------------------------------*)
-Lemma SIM_F_KE_CHAN f1 f2 γtoka γfraca γseca γsecb L :
+(*Lemma SIM_F_KE_CHAN f1 f2 γtoka γfraca γseca γsecb L :
     let LblThy := LblSecChannel γtoka atokN γfraca γseca γsecb in
     is_closed_expr ∅ f1 ->
     is_closed_expr ∅ f2 ->
@@ -176,7 +396,7 @@ Lemma SIM_F_KE_CHAN f1 f2 γtoka γfraca γseca γsecb L :
     ≤ (F_OAUTH channel2 (F_KE_L getKey2 channel2 leak2 (CHAN getKey2 channel2 f2))) <| LblEnvSec ++ L |> {{ (λ v1 v2, ⌜ v1 = v2 ⌝) }}.
 Proof.
 Admitted.   
-
+*)
 
   
   
